Adding for loop and proving equivalence of for and while

843/imp.v
@@ -1,48 +1,91 @@
-
 Require Import Omega.
+Require Import SfLib.
+Require Import Coq.Arith.Peano_dec.
+Require Import Coq.Arith.EqNat.
+Require Import Coq.Lists.List.
 
-Fixpoint ble_nat (n m : nat) : bool :=
-  match n with
-  | O => true
-  | S n' =>
-      match m with
-      | O => false
-      | S m' => ble_nat n' m'
-      end
-  end.
+Inductive id : Type :=
+| Id : nat -> id.
+
+Definition X : id := Id 0.
+Definition Y : id := Id 1.
+Definition Z : id := Id 2.
+
+Definition state := id -> nat.
+
+Theorem eq_id_dec : forall i j : id, {i = j} + {i <> j}.
+intros.
+destruct i. destruct j.
+destruct (eq_nat_dec n n0).
+left. rewrite e. reflexivity.
+right. intros contra. inversion contra. contradiction.
+Defined.
+
+Definition empty_state : state :=
+  fun _ => 0.
+
+Definition update (st : state) (i : id) (n : nat) : state :=
+  fun x => if (eq_id_dec x i) then n else (st i).
 
 Inductive aexp : Type :=
-  | ANum : nat -> aexp
-  | APlus : aexp -> aexp -> aexp
-  | AMinus : aexp -> aexp -> aexp
-  | AMult : aexp -> aexp -> aexp.
+| ANum : nat -> aexp
+| AId : id -> aexp
+| APlus : aexp -> aexp -> aexp
+| AMinus : aexp -> aexp -> aexp
+| AMult : aexp -> aexp -> aexp.
 
 Inductive bexp : Type :=
-  | BTrue : bexp
-  | BFalse : bexp
-  | BEq : aexp -> aexp -> bexp
-  | BLe : aexp -> aexp -> bexp
-  | BNot : bexp -> bexp
-  | BAnd : bexp -> bexp -> bexp.
+| BTrue : bexp
+| BFalse : bexp
+| BEq : aexp -> aexp -> bexp
+| BLe : aexp -> aexp -> bexp
+| BNot : bexp -> bexp
+| BAnd : bexp -> bexp -> bexp.
 
-Fixpoint aeval (a : aexp) : nat :=
+Inductive com : Type :=
+| CSkip : com
+| CBreak : com
+| CAss : id -> aexp -> com
+| CSeq : com -> com -> com
+| CIf : bexp -> com -> com -> com
+| CWhile : bexp -> com -> com
+| CFor : com -> bexp -> com -> com -> com.
+
+Notation "'SKIP'" :=
+  CSkip.
+Notation "'BREAK'" :=
+  CBreak.
+Notation "x '::=' a" :=
+  (CAss x a) (at level 60).
+Notation "c1 ;; c2" :=
+  (CSeq c1 c2) (at level 80, right associativity).
+Notation "'WHILE' b 'DO' c 'END'" :=
+  (CWhile b c) (at level 80, right associativity).
+Notation "'IFB' c1 'THEN' c2 'ELSE' c3 'FI'" :=
+  (CIf c1 c2 c3) (at level 80, right associativity).
+Notation "'FOR' c1 b c2 'DO' c3 'END'" :=
+  (CFor c1 b c2 c3) (at level 90, right associativity).
+
+Fixpoint aeval (st : state) (a : aexp) : nat :=
   match a with
   | ANum n => n
-  | APlus l r => (aeval l) + (aeval r)
-  | AMinus l r => (aeval l) - (aeval r)
-  | AMult l r => (aeval l) * (aeval r)
+  | AId i => st i       
+  | APlus l r => (aeval st l) + (aeval st r)
+  | AMinus l r => (aeval st l) - (aeval st r)
+  | AMult l r => (aeval st l) * (aeval st r)
   end.
 
-Fixpoint beval (b : bexp) : bool :=
+Fixpoint beval (st : state) (b : bexp) : bool :=
   match b with
   | BTrue => true
   | BFalse => false
-  | BEq l r => beq_nat (aeval l) (aeval r)
-  | BLe l r => ble_nat (aeval l) (aeval r)
-  | BNot x => negb (beval x)
-  | BAnd l r => andb (beval l) (beval r)
+  | BEq l r => beq_nat (aeval st l) (aeval st r)
+  | BLe l r => ble_nat (aeval st l) (aeval st r)
+  | BNot x => negb (beval st x)
+  | BAnd l r => andb (beval st l) (beval st r)
   end.
 
+(*
 Inductive aevalR : aexp -> nat -> Prop :=
   | E_ANum : forall n, aevalR (ANum n) n
   | E_APlus : forall x1 x2 v1 v2, (aevalR x1 v1) -> (aevalR x2 v2) -> (aevalR (APlus x1 x2) (v1 + v2))
@@ -70,15 +113,49 @@ intros H. induction H; try apply (aeval_iff_aevalR x1 v1) in H; try apply (aeval
 generalize dependent r.
 induction b; intros; subst; constructor; try apply (aeval_iff_aevalR a); try apply (aeval_iff_aevalR a0); try apply IHb; try apply IHb1; try apply IHb2; reflexivity.
 Qed.
+ *)
 
+Reserved Notation "c1 '/' st '||' st'" (at level 40, st at level 39).
 
+Inductive ceval : com -> state -> state -> Prop :=
+| E_Skip : forall st,
+             SKIP / st || st
+| E_Ass : forall st a1 n x,
+            aeval st a1 = n ->
+            (x ::= a1) / st || (update st x n)
+| E_Seq : forall c1 c2 st st' st'',
+            c1 / st || st' ->
+            c2 / st' || st'' ->
+            (c1 ;; c2) / st || st''
+| E_IfTrue : forall st st' b c1 c2,
+               beval st b = true ->
+               c1 / st || st' ->
+               (IFB b THEN c1 ELSE c2 FI) / st || st'
+| E_IfFalse : forall st st' b c1 c2,
+                beval st b = false ->
+                c2 / st || st' ->
+                (IFB b THEN c1 ELSE c2 FI) / st || st'
+| E_WhileEnd : forall b st c,
+                 beval st b = false ->
+                 (WHILE b DO c END) / st || st
+| E_WhileLoop : forall st st' st'' b c,
+                  beval st b = true ->
+                  c / st || st' ->
+                  (WHILE b DO c END) / st' || st'' ->
+                  (WHILE b DO c END) / st || st''
+| E_For : forall st st' st'' b c1 c2 c3,
+               c1 / st || st' ->
+               (WHILE b DO (c3 ;; c2) END) / st' || st'' ->
+               (CFor c1 b c2 c3) / st || st''
 
+  where "c1 '/' st '||' st'" := (ceval c1 st st').
 
-
-
-
-
-
-
-
-
+Theorem for_while_equiv : forall b c1 c2 c3 st1 st2,
+                            (CFor c1 b c2 c3) / st1 || st2 <->
+                            (c1 ;; CWhile b (c3 ;; c2)) / st1 || st2.
+Proof.
+  intros.
+  split; intros H1; inversion H1; subst;
+  [ apply E_Seq with (st' := st')
+  | apply E_For with (st' := st')]; assumption; assumption.
+Qed.
